coq/proof/AdequacyLocal.v
@@ -60,6 +60,7 @@ Inductive sim_local_stack
          (INCR: InvMem.Rel.le (InvMem.Rel.lift mem_src mem_tgt uniqs_src uniqs_tgt privs_src privs_tgt inv1) inv')
          (MEM: InvMem.Rel.sem conf_src conf_tgt mem'_src mem'_tgt inv')
          (RETVAL: TODO.lift2_option (genericvalues_inject.gv_inject inv'.(InvMem.Rel.inject)) retval'_src retval'_tgt)
+         (VALID: valid_retvals mem'_src mem'_tgt retval'_src retval'_tgt)
          (RETURN_SRC: return_locals
                         conf_src.(CurTargetData)
                         retval'_src id_src noret_src typ_src
@@ -190,8 +191,8 @@ Axiom callExternalOrIntrinsics_inject: forall
              (<<MEM: InvMem.Rel.sem (mkCfg S0 TD Ps0 Gs Fs0) (mkCfg S1 TD Ps1 Gs Fs1) Mem0' Mem1' invmem1>>)
              /\ (<<MEMLE: InvMem.Rel.le invmem0 invmem1>>)
              /\ (<<VAL_INJECT: option_f2 (genericvalues_inject.gv_inject (InvMem.Rel.inject invmem1))
-                                 oresult0 oresult1>>))
-
+                                 oresult0 oresult1>>)
+             /\ (<<VALID: valid_retvals Mem0' Mem1' oresult0 oresult1>>))
 .
 
 Lemma sim_local_stack_invmem_le
@@ -282,6 +283,10 @@ Proof.
           instantiate (1:= Some _).
           eassumption.
         }
+        {
+          exploit RET; eauto. i; des.
+          admit. (* free-allocas preserves valid_ptr *)
+        }
         { ss. }
         clear LOCAL. intro LOCAL. des. simtac.
 
@@ -329,6 +334,9 @@ Proof.
         { instantiate (2:= Some _).
           instantiate (1:= Some _).
           eassumption.
+        }
+        { exploit RET; eauto. i; des.
+          admit. (* ditto *)
         }
         { ss. des_ifs. }
         clear LOCAL. intro LOCAL. des. simtac.
@@ -394,6 +402,7 @@ Proof.
           instantiate (1:= Some _).
           ss. (* it may put existential goals as nil/nil, but I don't care. It's return void *)
         }
+        { econs; eauto; ss. }
         { ss. }
         clear LOCAL. intro LOCAL. des. simtac.
 
@@ -631,9 +640,7 @@ Proof.
         } des.
 
         hexploit RETURN; eauto.
-        { instantiate (1:= oresult0).
-          inv VAL_INJECT; ss.
-        }
+        { inv VAL_INJECT; ss. }
         clear RETURN. intro RETURN. des.
 
         rewrite exCallUpdateLocals_spec in *.
@@ -696,4 +703,4 @@ Unshelve.
 { by econs; eauto. }
 (* { by econs; eauto. } *)
 (* { by econs; eauto. } *)
-Qed.
+Admitted.
