coq/proof/SoundPostcondCall.v
@@ -278,6 +278,7 @@ Lemma postcond_call_sound
                                             invmem0) invmem1)
       (MEM: InvMem.Rel.sem conf_src conf_tgt mem1_src mem1_tgt invmem1)
       (RETVAL: TODO.lift2_option (genericvalues_inject.gv_inject invmem1.(InvMem.Rel.inject)) retval1_src retval1_tgt)
+      (VALID: valid_retvals mem1_src mem1_tgt retval1_src retval1_tgt)
       (RETURN_SRC: return_locals
                      conf_src.(CurTargetData)
                      retval1_src id_src noret_src typ_src
